examples/refinement/HighComp.fst
@@ -1,0 +1,43 @@
+module HighComp
+
+module U32 = FStar.UInt32
+  
+type mint = U32.t
+type state = mint * mint
+//type state = int
+let comp a = state -> M (a * state)
+
+val hreturn : (a:Type) -> a -> comp a
+let hreturn (a:Type) (x : a) = fun s -> (x, s)
+
+val hbind : (a:Type) -> (b:Type) -> comp a -> (a -> comp b) -> comp b
+let hbind (a:Type) (b:Type) (m : comp a) (f : a -> comp b) = 
+    fun s -> let (a, s1) = m s in f a s1
+
+val hread : i:int -> comp mint
+let hread (i:int) : comp mint = 
+    fun s -> if i = 0 then (fst s, s) 
+          else (snd s, s)
+
+val hwrite : i:int -> v:mint -> comp unit
+let hwrite (i:int) (v:mint) : comp unit =
+    fun s -> if i = 0 then ((), (v, snd s))
+          else ((), (fst s, v))
+
+val dread : unit -> comp state
+let dread (_ : unit) : comp state = fun s -> (s, s) 
+
+val dwrite : v:state -> comp unit
+let dwrite (v : state) : comp unit = fun s -> ((), v)
+
+// NOTE : ommiting type annotations from dread and dwrite defs
+// makes the effect definition fail
+
+total reifiable reflectable new_effect {
+      HIGH : a:Type -> Effect
+      with repr  = comp 
+       ; bind     = hbind
+       ; return   = hreturn
+       ; get      = hread
+       ; put      = hwrite
+       }
